OVN_template

ovn/src/ovn_template.rs
@@ -1,0 +1,123 @@
+use hacspec_lib::*;
+
+pub trait Group {
+    type group_type : PartialEq;
+
+    const q : usize; // Prime order
+    const g : Self::group_type; // Generator (elemnent of group)
+
+    fn g_pow(x : usize) -> Self::group_type;
+    fn one() -> Self::group_type;
+    fn prod(x : Self::group_type, y : Self::group_type) -> Self::group_type;
+    fn div(x : Self::group_type, y : Self::group_type) -> Self::group_type;
+    fn random_element() -> Self::group_type;
+}
+
+struct eligible_votes {
+    v_id : usize,
+}
+
+const n : usize = 3;
+const P : [eligible_votes; 3] = // n = 3
+    [eligible_votes {v_id: 0},
+     eligible_votes {v_id: 1},
+     eligible_votes {v_id: 2}];
+
+pub fn select_private_voting_key<G : Group> (random : usize) -> usize {
+    random % G::q // x_i \in_R Z_q;
+}
+
+pub fn ZKP<G : Group>(xi : usize) -> usize {
+    // TODO: Non-usizeeractive Schnorr proof using Fiat-Shamir heuristics
+    0
+}
+
+// State of bulletin board
+pub fn get_broadcast1() -> (Vec<usize>, Vec<usize>) {
+    (Vec::new(), Vec::new())
+}
+
+pub fn check_valid(zkp : usize) -> bool {
+    true
+}
+
+pub fn broadcast1<G : Group>(xi : G::group_type, zkp : usize, i : usize) {
+
+}
+
+pub fn register_vote<G : Group>(i : usize, random : usize) {
+    let xi = select_private_voting_key::<G>(random);
+    broadcast1::<G>(G::g_pow(xi), ZKP::<G>(xi), i);
+    let (gs, zkps) = get_broadcast1();
+
+    for zkp in zkps {
+        check_valid(zkp);
+    }
+
+    let mut prod1 = G::one();
+    for j in 1..i-1 {
+        prod1 = G::prod(prod1, G::g_pow(gs[j]));
+    }
+    let prod2 = G::one();
+    for j in i+1..n {
+        prod1 = G::prod(prod1, G::g_pow(gs[j]));
+    }
+    let Yi = G::div(prod1, prod2);
+    // implicityly: Y_i = g^y_i
+}
+
+// Meta Round:
+
+// pub fn round1(user){
+//     for x in user {
+//         register()
+//     }
+// }
+
+// Cramer, Damgård and Schoenmakers (CDS) technique
+pub fn ZKP_one_out_of_two(vi : bool) -> usize {
+    32 // TODO
+}
+
+pub fn broadcast2<G : Group> (g_pow_xiyi : G::group_type, g_pow_vi : G::group_type, g_pow_vi_zkp : usize) {
+
+}
+
+pub fn get_broadcast2<G : Group> () -> (Vec<G::group_type>,Vec<G::group_type>,Vec<usize>) {
+    (Vec::new(),Vec::new(),Vec::new())
+}
+
+pub fn cast_vote<G : Group>(xi : usize, yi : usize, vi : bool) {
+    broadcast2::<G>(G::g_pow(xi * yi), G::g_pow(if vi { 1 } else { 0 }), ZKP_one_out_of_two(vi));
+}
+
+// Meta Round:
+
+// pub fn round2(){
+//     for x in user {
+//         cast_vote()
+//     }
+// }
+
+pub fn tally_votes<G : Group>() -> usize {
+    let (g_pow_xi_yi, g_pow_vi, zkps) = get_broadcast2::<G>();
+    for zkp in zkps {
+        check_valid(zkp);
+    }
+
+    let mut vote_result = G::one();
+    for (gxiyi, gvi) in g_pow_xi_yi.into_iter().zip(g_pow_vi) {
+        vote_result = G::prod(vote_result, G::prod(gxiyi, gvi));
+    }
+
+    let mut tally = 0;
+    for i in 1..n { // Should be while, but is bounded by n anyways!
+        if G::g_pow(tally) != vote_result {
+            tally += 1
+        }
+        else {
+            return tally
+        }
+    }
+    tally
+}
