ovn/proofs/ssprove/extraction/ovn_eq_proof.v
@@ -1,36 +1,36 @@
 Set Warnings "-notation-overridden,-ambiguous-paths".
 From mathcomp Require Import all_ssreflect.
 
-From JasminSSProve Require Import jasmin_translate.
+(* From JasminSSProve Require Import jasmin_translate. *)
 From Crypt Require Import Prelude Package pkg_composition.
-From Crypt Require Import Axioms. (* proof_irrelevance *)
 From extructures Require Import ord fset fmap.
 Import PackageNotation.
+From Coq Require Import ZArith.
+(* #[global] Hint Resolve preceq_I preceq_O preceq_refl : preceq. *)
 
-#[global] Hint Resolve preceq_I preceq_O preceq_refl : preceq.
-
-Definition pdisj (P : precond) (s_id : p_id) (rhs : {fset Location}) :=
-  (forall h1 h2 l a v s_id', l = translate_var s_id' v -> (s_id ⪯ s_id') -> (P (h1, h2) -> P (set_heap h1 l a, h2))) /\
+Definition pdisj (P : precond) (* (s_id : p_id) *) (rhs : {fset Location}) :=
+  (forall h1 h2 l a (* v *) (* s_id' *), (* l = translate_var s_id' v -> (s_id ⪯ s_id') -> *) (P (h1, h2) -> P (set_heap h1 l a, h2))) /\
     (forall h1 h2 l a, l \in rhs -> (P (h1, h2) -> P (h1, set_heap h2 l a))).
 
 (* From Crypt Require Import choice_type Package Prelude. *)
+From Crypt Require Import Axioms.
 
-Require Import Hacspec_ovn_Schnorr_Random_oracle.
+(* Require Import Hacspec_ovn_Schnorr_Random_oracle. *)
 
 Require Import SigmaProtocol.
 Require Import DDH.
 
-Require Import Hacspec_ovn_Schnorr.
-
+(* Require Import Hacspec_ovn_Schnorr. *)
 Require Import Schnorr.
 
 Require Import Hacspec_ovn.
+Require Import OVN.
 
 From Hacspec Require Import ChoiceEquality.
 (* From Hacspec Require Import Hacspec_Lib_Pre. *)
 From Hacspec Require Import Hacspec_Lib.
 
-Module Schnorr_eq (GP : GroupParam).
+Module Schnorr_eq (GP : GroupParam)  (OP : OVNParam).
   Import GP.
   Module Sigma1 := Schnorr GP.
   Module RO1 := Sigma1.Sigma.Oracle.
@@ -40,9 +40,26 @@ Module Schnorr_eq (GP : GroupParam).
   (* Check (chProd Sigma1.MyAlg.choiceStatement Sigma1.MyAlg.choiceWitness). *)
   Locate choiceTranscript.
 
-  Definition Schnorr_translate_type (x : Sigma1.MyAlg.choiceStatement × Sigma1.MyAlg.choiceWitness) : t_Relation :=
-    (Hacspec_Lib_Pre.repr _ (word.modulus (nat_of_ord (fst x))),
-      Hacspec_Lib_Pre.repr _ (word.modulus (nat_of_ord (snd x) ))).
+  Notation mymod := (4002409555221667393417789825735904156556882819939007885332058136124031650490837864442687629129015664037894272559787)%Z.
+  Axiom mymod_is_statement : Z.to_nat mymod = #|Sigma1.MyParam.Statement|.
+
+  Notation mymod2 := (9574)%Z.
+  Axiom mymod2_is_statement : Z.to_nat mymod2 = #|Sigma1.MyParam.Witness|.
+  
+  Definition Schnorr_translate_type (x : Sigma1.MyAlg.choiceStatement × Sigma1.MyAlg.choiceWitness) : t_Relation.
+  Proof.
+    refine (cast_ord _ (fst x), cast_ord _ (snd x)).
+    unfold pos.
+    rewrite mymod_is_statement.
+    symmetry.
+    eapply prednK.
+    apply Sigma1.MyParam.positive_gT.
+
+    rewrite mymod2_is_statement.
+    symmetry.
+    eapply prednK.
+    apply Sigma1.MyParam.Witness_pos.
+  Defined.
 
   Ltac destruct_pre :=
     repeat
@@ -68,31 +85,141 @@ Module Schnorr_eq (GP : GroupParam).
           destruct H as [o]
       end; simpl in *; subst.
 
-  Ltac remove_get_in_lhs :=
-    eapply better_r_get_remind_lhs ;
-    unfold Remembers_lhs , rem_lhs ;
-    [ intros ? ? ? ;
-      destruct_pre ;
-      repeat (rewrite get_set_heap_neq ; [ | apply injective_translate_var3 ; reflexivity ]) ;
-      rewrite get_set_heap_eq ;
-      reflexivity | ].
+  (* Ltac remove_get_in_lhs := *)
+  (*   eapply better_r_get_remind_lhs ; *)
+  (*   unfold Remembers_lhs , rem_lhs ; *)
+  (*   [ intros ? ? ? ; *)
+  (*     destruct_pre ; *)
+  (*     repeat (rewrite get_set_heap_neq ; [ | apply injective_translate_var3 ; reflexivity ]) ; *)
+  (*     rewrite get_set_heap_eq ; *)
+  (*     reflexivity | ]. *)
 
-  From Crypt Require Import Axioms.
+  Definition uniform_secret (x : Arit (uniform (H := Sigma1.MyParam.Witness_pos) #|Sigma1.MyParam.Witness|)) : t_Secret.
+  Proof.
+    simpl in x.
+    
+    refine (cast_ord _ x).
+    rewrite mymod2_is_statement.
+    simpl.
+    symmetry.
+    eapply prednK.
+    apply Sigma1.MyParam.Witness_pos.
+  Defined.    
+    (* Hacspec_Lib_Pre.repr _ (word.modulus (nat_of_ord x)). *)
 
-  Check proof_irrelevance.
-
-  Lemma both_eq : forall {A : choice_type} {L I} (a b : both L I A),
-      both_prog a = both_prog b ->
-      a = b.
+  Theorem random_sample (pre : precond) :
+    forall i `{Positive i},
+    exists (random_val : Arit (uniform i)),
+      ⊢ ⦃ pre ⦄
+          x ← sample uniform i ;; ret x ≈ ret random_val
+                                      ⦃ fun '(v0, h0) '(v1, h1) => pre (h0, h1) ⦄.
   Proof.
     intros.
-    destruct a , b.
-    cbn in *. subst.
-    f_equal ; apply proof_irrelevance.
+    eexists.
+    apply (r_const_sample_L _ (fun x => ret x) _).
+    apply LosslessOp_uniform.
+    intros.
+    apply r_ret.
+    intros.
+    apply H0.
+    Unshelve.
+    refine (Ordinal (n:={| pos := i; cond_pos := H |}) (m := 0) _).
+    easy.
   Qed.
 
-  Lemma bind_ret_both : forall {A B : choice_type} {L I} `{fsubset_loc : is_true (fsubset (fset [::]) L)} `{fsubset_opsig : is_true (fsubset (fset [::]) I)} (f : A -> both L I B) (x : A),
-      (bind_both (fsubset_loc := fsubset_loc) (fsubset_opsig := fsubset_opsig) (ret_both x) f) = f x.
+  (* Definition cast_type (x : (chProd (chProd (chProd t_G t_G) t_Q) t_Q)) : (tgt *)
+  (*            (@pair ident (prod choice_type choice_type) Sigma1.Sigma.RUN *)
+  (*               (@pair choice_type choice_type *)
+  (*                  (chProd Sigma1.MyAlg.choiceStatement *)
+  (*                     Sigma1.MyAlg.choiceWitness) *)
+  (*                  Sigma1.MyAlg.choiceTranscript))). *)
+  (* Proof. *)
+  (*   destruct x as [[[]]]. *)
+  (*   repeat split. *)
+  (*   refine (Ordinal (m := Z.to_nat (Hacspec_Lib_Pre.unsigned s)) _). *)
+  (*   simpl. *)
+Theorem better_rsame_head_cmd_alt :
+  forall {A B C : choiceType} {f₀  : A -> raw_code B}  {f₁ : A -> raw_code C}
+    (m : command A) pre (post : postcond B C),
+    ⊢ ⦃ pre ⦄
+      x ← cmd m ;; ret x ≈ x ← cmd m ;; ret x
+    ⦃ fun '(a₀, s₀) '(a₁, s₁) => pre (s₀, s₁) /\ a₀ = a₁ ⦄ ->
+    (forall a, ⊢ ⦃ pre ⦄ f₀ a ≈ f₁ a ⦃ post ⦄) ->
+    ⊢ ⦃ pre ⦄ x ← cmd m ;; f₀ x ≈ x ← cmd m ;; f₁ x ⦃ post ⦄.
+Proof.
+  intros A B C f₀ f₁ m pre post hm hf.
+  eapply from_sem_jdg. rewrite !repr_cmd_bind.
+  eapply (RulesStateProb.bind_rule_pp (repr_cmd m) (repr_cmd m)).
+  - eapply to_sem_jdg in hm. rewrite !repr_cmd_bind in hm.
+    rewrite bindrFree_ret in hm. eauto.
+  - intros a₀ a₁. eapply to_sem_jdg.
+    eapply rpre_hypothesis_rule.
+    intros s₀ s₁ [h e]. subst.
+    eapply rpre_weaken_rule. 1: eapply hf.
+    simpl. intros ? ? [? ?]. subst. auto.
+Qed.
+    
+  Lemma better_r_const_sample_R :
+  forall {A B : choiceType} (op : Op) c₀ c₁ (pre : precond) (post : postcond A B),
+    LosslessOp op ->
+    (forall x, ⊢ ⦃ pre ⦄ c₀ ≈ c₁ x ⦃ post ⦄) ->
+    ⊢ ⦃ pre ⦄ c₀ ≈ x ← sample op ;; c₁ x ⦃ post ⦄.
+Proof.
+  intros A B op c₀ c₁ pre post hop h.
+  eapply r_transL with (x ← sample op ;; (fun _ => c₀) x).
+  - apply r_dead_sample_L. 1: auto.
+    apply rreflexivity_rule.
+  - apply (better_rsame_head_cmd_alt (cmd_sample op)).
+    + eapply rpre_weaken_rule. 1: eapply cmd_sample_preserve_pre.
+      auto.
+    + apply h.
+Qed.
+
+  (* Ltac solve_var_neq := *)
+  (*   ((now apply injective_translate_var3) || *)
+  (*            (apply injective_translate_var2 ; red ; intros ; subst)). *)
+  (* Ltac eexists_set_heap := *)
+  (*   eexists ; split ; [ | *)
+  (*   match goal with *)
+  (*   | [ |- context [ *)
+  (*             set_heap _ _ ?d *)
+  (*             = set_heap _ _ ?d *)
+  (*     ] ] => *)
+  (*       reflexivity *)
+  (*   end || *)
+  (*       match goal with *)
+  (*       | [ |- context [ *)
+  (*                 set_heap ?a ?b ?c *)
+  (*                 = set_heap _ _ ?e *)
+  (*         ] ] => *)
+  (*           rewrite [set_heap a b c]set_heap_commut ; [ reflexivity | *)
+  (*           solve_var_neq ] *)
+  (*       end]. *)
+
+  Ltac solve_in :=
+    repeat match goal with
+           | |- is_true (?v \in fset1 ?v :|: _) => apply/fsetU1P; left; auto
+           | |- is_true (_ \in fsetU _ _) => apply/fsetU1P; right
+           end.
+
+  Ltac pdisj_apply h :=
+    lazymatch goal with
+    | |- ?pre (set_heap _ _ _, set_heap _ _ _) => eapply h; [ solve_in | pdisj_apply h ]
+    | |- ?pre (set_heap _ _ _, _) =>
+        eapply h ; [ reflexivity | auto with preceq | pdisj_apply h ]
+    | |- _ => try assumption
+    end.
+
+
+  Ltac solve_in_fset :=
+    rewrite in_fset ; repeat (reflexivity || (rewrite mem_head) || (now rewrite Bool.orb_true_r) || (now rewrite Bool.orb_true_l) || rewrite in_cons ; simpl).
+
+  Theorem unfold_prod0 :
+    forall L I A (x : both L I A), prod_to_prod_n 0 x = x.
+  Proof. destruct A ; reflexivity. Qed.
+
+  Lemma bind_solve_lift_ret_both : forall {A B : choice_type} {L1 L2 I1 I2} `{fsubset_loc : is_true (fsubset (fset [::]) L1)} `{fsubset_opsig : is_true (fsubset (fset [::]) I1)} `{fsubset_loc2 : is_true (fsubset L1 L2)} `{fsubset_opsig2 : is_true (fsubset I1 I2)} (f : A -> both L2 I2 B) (x : A),
+      (bind_both (L1 := L1)  (I1 := I1) (fsubset_loc := fsubset_loc2) (fsubset_opsig := fsubset_opsig2) (lift_both (fsubset_loc := fsubset_loc) (fsubset_opsig := fsubset_opsig) (ret_both x)) f) = f x.
   Proof.
     intros.
     apply both_eq.
@@ -103,123 +230,408 @@ Module Schnorr_eq (GP : GroupParam).
     destruct both_prog. simpl.
     reflexivity.
   Qed.
+
+  Lemma bind_solve_both_assoc :
+    forall {A B : choice_type} {L1 L2 I1 I2} (f : A -> both L2 I2 B) (x : A) `{fsubset_loc : is_true (fsubset (fset [::]) L1)} `{fsubset_opsig : is_true (fsubset (fset [::]) I1)} `{fsubset_loc2 : is_true (fsubset L1 L2)} `{fsubset_opsig2 : is_true (fsubset I1 I2)},
+      (bind_both (fsubset_loc := fsubset_loc2) (fsubset_opsig := fsubset_opsig2) (lift_both (L2 := L1) (I2 := I1) (fsubset_loc := fsubset_loc) (fsubset_opsig := fsubset_opsig) (ret_both x)) f) =
+      (bind_both (fsubset_loc := fsubset_trans fsubset_loc fsubset_loc2) (fsubset_opsig := fsubset_trans fsubset_opsig fsubset_opsig2) (ret_both x) f).
+  Proof.
+    intros.
+    apply both_eq.
+    simpl.
+    unfold bind_raw_both.
+    simpl.
+    destruct (f x). simpl.
+    destruct both_prog. simpl.
+    reflexivity.
+  Qed.
+
+  Theorem unfold_letb'2 :
+    forall L1 L2 I1 I2 A B C,
+    forall (z : both L1 I1 (A × B)) (f : _ -> both L2 I2 C),
+    forall `{fsubset_loc1 : is_true (fsubset (fset [::]) L1)} `{fsubset_opsig1 : is_true (fsubset (fset [::]) I1)},
+    forall `{fsubset_loc2 : is_true (fsubset L1 L2)} `{fsubset_opsig2 : is_true (fsubset I1 I2)},
+      is_state (lift_n (fsubset_loc := fsubset_loc2) (fsubset_opsig := fsubset_opsig2) 1 z f) =
+        ('(x, y) ← is_state z ;; is_state (f (lift_both (fsubset_loc := fsubset_loc1) (fsubset_opsig := fsubset_opsig1) (ret_both x) : both _ _ A, lift_both (fsubset_loc := fsubset_loc1) (fsubset_opsig := fsubset_opsig1) (ret_both y) : both _ _ B))).
+  Proof.
+    intros.
+    unfold lift_n at 1.
+    simpl.
+
+    f_equal.
+    apply functional_extensionality.
+    intros [].
+
+    rewrite unfold_prod0.
+
+    rewrite <- surjective_pairing.
+    set (prod_to_prod _).
+    set (solve_lift _, solve_lift _).
+    replace p with p0 ; [ reflexivity | subst p p0 ].
+
+    unfold prod_to_prod at 1.
+
+    rewrite bind_solve_both_assoc.
+    rewrite bind_solve_both_assoc.
+
+    rewrite bind_ret_both.
+    rewrite bind_ret_both.
+
+    simpl.
+
+    f_equal.
+    f_equal.
+    apply proof_irrelevance.
+    apply proof_irrelevance.
+    f_equal.
+    f_equal.
+    apply proof_irrelevance.
+    apply proof_irrelevance.
+  Qed.
   
-  Theorem Schnorr_eq_proof id0 (pre : precond)  :
+  Theorem Schnorr_eq_proof (* id0 *) (pre : precond)  :
     forall (hw : (Sigma1.MyAlg.choiceStatement × Sigma1.MyAlg.choiceWitness)),
-    (pdisj pre id0 (fset0)) ->
+    forall (H_pdisj : pdisj pre (* id0 *) (fset [ :: RO1.queries_loc ; Sigma1.MyAlg.commit_loc ])),
+      forall (* exists *) (random_sample1 : Arit (uniform (H := Sigma1.MyParam.Witness_pos) Sigma1.MyAlg.i_witness)) random_sample2,
     ⊢ ⦃ pre ⦄
-        is_state (both_prog (fiat_shamir_run (ret_both (Schnorr_translate_type hw))))
+        is_state (both_prog (fiat_shamir_run (ret_both (Schnorr_translate_type hw)) (ret_both (uniform_secret random_sample1)) (ret_both random_sample2)))
         ≈
         get_op_default (Sigma1.Sigma.Fiat_Shamir ∘ RO1.RO) (Sigma1.Sigma.RUN, ((chProd Sigma1.MyAlg.choiceStatement Sigma1.MyAlg.choiceWitness), Sigma1.MyAlg.choiceTranscript)) hw
         ⦃ fun '(v0, h0) '(v1, h1) => pre (h0, h1) ⦄.
   Proof.
     intros.
-    
+    (* eexists. *)
+    (* eexists. *)
+
     (* Unfolding and simplifying to raw code! *)
     (* TODO: Work on higher level than raw code? *)
-    
+
     rewrite get_op_default_link.
     erewrite get_op_default_spec.
-    2: {
-      cbn.
-      done.
-    }
+    2: {cbn. done.}
     ssprove_code_simpl.
-
-    rewrite fiat_shamir_run_equation_1.
     destruct hw.
-
+    hnf.
+    rewrite fiat_shamir_run_equation_1.
+    
     ssprove_code_simpl.
     ssprove_code_simpl_more.
 
+    (* Ltac get_next_statement := _. *)
     unfold let_both at 1.
-
-    unfold prod_to_prod_n at 1 ; fold @prod_to_prod_n ; rewrite prod_to_prod_equation_1 ; rewrite !bind_ret_both ; simpl.
-    unfold Schnorr_translate_type ; simpl.
-    rewrite v_Commit_equation_1.
-
-    unfold Build_t_G at 1.
-
+    rewrite unfold_letb'2.
+    rewrite bind_rewrite.
+    destruct Schnorr_translate_type eqn:So.
+    unfold let_both at 1.
+    unfold let_both at 1.
+    unfold let_both at 1.
+    unfold let_both at 1.
+    unfold let_both at 1.
+    rewrite unfold_letb'2.
     
-    unfold is_state , both_prog.
-    rewrite !let_both_equation_1.
-    unfold both_prog.
-    rewrite !prod_both_equation_1.
-    setoid_rewrite bind_assoc.
-    setoid_rewrite bind_assoc.
-    setoid_rewrite bind_assoc.
-    setoid_rewrite bind_assoc.
-    (* unfold is_state, ret_both, lift_both, both_prog, bind_both, bind_raw_both. *)
-
-    (* Actual proof *)
-
     match goal with
     | [ |- context [ ⊢ ⦃ ?P ⦄ ?x ≈ assertD ?b ?f ⦃ ?Q ⦄ ] ] =>
         change x with (assertD true (fun _ => x)) ;
         apply (r_assertD true b pre _ (fun _ => x))
     end.
     {
+      clear -So.
       intros.
+      apply pair_equal_spec in So.
+      destruct So.
+      
+      eapply (@f_equal _ _ (cast_ord (esym _)) _ _) in H0.
+      erewrite cast_ordK in H0.
+      unfold fst in H0.
+      rewrite H0 ; clear H0.
+
+      eapply (@f_equal _ _ (cast_ord (esym _)) _ _) in H1.
+      erewrite cast_ordK in H1.
+      unfold snd in H1.
+      rewrite H1 ; clear H1.
+      clear.
+
+      destruct s1 , s2.
+      cbn.
+      unfold cast_ord.
+
+
+      unfold Sigma1.MyParam.R.
+      cbn.
+      pose nth_ord_enum.
+      unfold enum.
+      cbn.
+      simpl.
+      setoid_rewrite nth_ord_enum.
       admit.
     }
-    intros.
-    
-    match goal with
-    | [ |- context [ ⊢ ⦃ ?P ⦄ bind ?a ?f ≈ pkg_core_definition.sampler ?x ?y ⦃ ?Q ⦄ ] ] =>
-        set (a) ; set (f) ; set (x) ; set (y)
-    end.
-    Check pkg_core_definition.sampler o.
-    pose (Arit o).
-    cbn in t.
-    pose Sigma1.MyAlg.i_witness.
-    cbn in n.
-    
-    assert (s1 : forall (x : Arit o), commit_loc).
-    { clear. intros.
-      apply (Schnorr_translate_type).
-      split.
-      (* apply (Hacspec_Lib_Pre.repr _ (word.modulus 1%nat)). *)
-      2:{
-        apply x.
-      }.
-      admit.
-    }
-    replace (x ← r ;; r0 _) with (x ← sample o ;; r0 (s1 x)) by admit.
-    apply r_uniform_bij with (f := id).
+    intros _ ?.
+    apply (better_r_const_sample_R) ; [ apply LosslessOp_uniform | intros ].
+
+    unfold random_oracle_query at 1.
+
+    rewrite bind_assoc.
+    rewrite bind_assoc.
+    rewrite bind_rewrite.
+
+    apply better_r_put_rhs.
+    apply better_r_put_get_rhs.
+    apply better_r_put_rhs.
+
+    rewrite emptymE.
+
+    rewrite bind_assoc.
+    rewrite bind_assoc.
+    rewrite bind_assoc.
+    rewrite bind_rewrite.
+    rewrite bind_assoc.
+    rewrite bind_assoc.
+
+    (* Sample *)
+    apply (better_r_const_sample_R) ; [ apply LosslessOp_uniform | intros ].
+    rewrite bind_rewrite.
+
+    unfold is_state at 1, both_prog at 1.
+    unfold bind ; fold @bind.
+    apply better_r_put_get_lhs.
+    apply better_r_put_lhs.
+
+    rewrite bind_rewrite.
+    rewrite bind_rewrite.
+
+    unfold prod_to_prod_n at 1 ; fold @prod_to_prod_n.
+    rewrite bind_rewrite.
+    rewrite bind_rewrite.
+
+    rewrite emptymE.
+    rewrite bind_assoc.
+    rewrite bind_assoc.
+    rewrite bind_rewrite.
+    apply better_r_put_rhs.
+
+    apply better_r.
+    apply r_get_remind_rhs with (v := x).
     {
-      apply injF_bij.
-      apply inj_id.
+      unfold Remembers_rhs  , rem_rhs.
+      intros ? ? ?.
+      clear -H.
+      destruct_pre.
+      rewrite get_set_heap_neq ; [ | easy ].
+      rewrite get_set_heap_neq ; [ | easy ].
+      rewrite get_set_heap_eq. reflexivity.
     }
+    apply better_r.
+
+    repeat (rewrite !bind_assoc ; rewrite bind_rewrite).
+    unfold is_state at 1, both_prog at 1.
+    unfold bind ; fold @bind.
+
+    apply better_r_put_get_lhs.
+    apply better_r_put_lhs.
+
+    rewrite bind_rewrite.
+    rewrite bind_rewrite.
+
+    unfold prod_to_prod_n at 1 ; fold @prod_to_prod_n.
+
+    rewrite bind_rewrite.
+    rewrite bind_assoc.
+    rewrite bind_rewrite.
+    rewrite bind_rewrite.
+    unfold prod_to_prod_n at 1 ; fold @prod_to_prod_n.
+    rewrite !unfold_prod0.
+    rewrite bind_assoc.
+    rewrite bind_assoc.
+    rewrite bind_rewrite. 
+    rewrite bind_rewrite. 
+    rewrite bind_assoc.
+    rewrite bind_rewrite. 
+    rewrite bind_rewrite. 
+
+    unfold prod_both at 1.
+    unfold prod_both at 1.
+    unfold prod_both at 1.
+    unfold is_state.
+    setoid_rewrite bind_assoc.
+    setoid_rewrite bind_assoc.
+    setoid_rewrite bind_assoc.
+    setoid_rewrite bind_assoc.
+    rewrite bind_rewrite.
+    unfold both_prog at 1 , is_state at 1.
+    unfold bind ; fold @bind.
+
+    apply better_r_put_get_lhs.
+    apply better_r_put_lhs.
+
+    rewrite bind_rewrite.
+    rewrite bind_rewrite.
+
+
+    rewrite bind_assoc.
+    rewrite bind_rewrite.
+    rewrite bind_rewrite.
+    apply r_ret.
+
     intros.
-    subst r0 r1.
+
+    clear -H H_pdisj.
+    destruct_pre.
+
+    repeat apply H_pdisj.
+    - solve_in_fset.
+    - solve_in_fset.
+    - solve_in_fset.
+    - assumption.
+
+      Unshelve.
+      all: intros ? ? ? ? ; apply proof_irrelevance.
+  Admitted.
+
+  Definition Schnorr_translate_type2 (x : Sigma1.MyAlg.choiceTranscript) : t_Transcript.
+  Proof.
+    destruct x as [[[]]].
+    refine (cast_ord _ s, cast_ord _ s0, cast_ord _ s1, cast_ord _ s2).
+    unfold pos.
+    rewrite mymod_is_statement.
+    symmetry.
+    eapply prednK.
+    apply Sigma1.MyParam.positive_gT.
+
+    unfold pos.
+    rewrite mymod_is_statement.
+    symmetry.
+    eapply prednK.
+    apply Sigma1.MyParam.positive_gT.
+
+    rewrite mymod2_is_statement.
+    symmetry.
+    eapply prednK.
+    apply Sigma1.MyParam.Witness_pos.
+
+    rewrite mymod2_is_statement.
+    symmetry.
+    eapply prednK.
+    apply Sigma1.MyParam.Witness_pos.
+  Defined.
+
+  Module OVN_mod := OVN GP OP.
+  Import OVN_mod.
+  Module OVN_proof (π2 : CDSParams) (Alg2 : SigmaProtocolAlgorithms π2).
+  Module OVN_OVN_mod := OVN π2 Alg2.
+  Import OVN_OVN_mod.
+
+  Theorem Schnorr__eq_proof (* id0 *) (pre : precond)  :
+    forall (hw : Sigma1.MyAlg.choiceTranscript),
+    forall (H_pdisj : pdisj pre (* id0 *) (fset [ :: RO1.queries_loc ; Sigma1.MyAlg.commit_loc ])),
+      (* forall i b, *)
+      forall (* exists *) (random_sample1 : Arit (uniform _)),
+    ⊢ ⦃ pre ⦄
+        is_state (both_prog (fiat_shamir_verify (ret_both (Schnorr_translate_type2 hw)) (ret_both (uniform_secret random_sample1))))
+        ≈
+        get_op_default ((Sigma1.Sigma.Fiat_Shamir ∘ RO1.RO)) (Sigma1.Sigma.VERIFY, ((Sigma1.MyAlg.choiceTranscript, 'bool))) hw
+        ⦃ fun '(v0, h0) '(v1, h1) => pre (h0, h1) ⦄.
+  Proof.
+        intros.
+    (* eexists. *)
+    (* eexists. *)
+
+    (* Unfolding and simplifying to raw code! *)
+    (* TODO: Work on higher level than raw code? *)
+
+    rewrite get_op_default_link.
+    erewrite get_op_default_spec.
+    2: {cbn. done.}
+    ssprove_code_simpl.
+    destruct hw as [[[]]].
     hnf.
+    rewrite fiat_shamir_verify_equation_1.
+    
+    ssprove_code_simpl.
+    ssprove_code_simpl_more.
+
+    (* setoid_rewrite bind_rewrite. *)
+
+    unfold prod_to_prod_n at 1 ; fold @prod_to_prod_n ; rewrite !unfold_prod0.
+    autorewrite with let_both.
+    autorewrite with prod_to_prod.
+    rewrite prod_assoc_equation_1.
+    
+    rewrite !bind_ret_both.
+
+    rewrite !bind_solve_both_assoc.
+    rewrite !bind_ret_both.
+    rewrite !bind_solve_both_assoc.
+    rewrite !bind_ret_both.
+    
+    unfold fst, snd.
+
+    unfold Schnorr_translate_type2.
+
+    unfold prod_to_prod_n at 2 ; fold @prod_to_prod_n.
+
+    (* Unset Printing Notations. *)
+    (* Set Printing Coercions. *)
+    match goal with
+    | |- context [let 'pair _ _ := prod_to_prod_n 1 ?b in ?x] =>
+        pose (is_state (both_prog (let 'pair _ _ := prod_to_prod_n 1 b in x)));
+        pose ('(_, _) ← is_state (both_prog b) ;; is_state (both_prog x))
+        ; set (b) ; set (x)
+    end.
+
+    epose (is_state (both_prog b) ;; _).
+
+    epose (_ ← (is_state b) ;; _).
+
+    assert (forall L1 I1 A B L2 I2 C (b : both L1 I1 (A × B)) (x : both L2 I2 C),
+               is_state (letb '(_, _) := b in x) =
+              '(_, _) ← is_state b ;; is_state x).
+    {
+      clear.
+      intros.
+      destruct b.
+      destruct both_prog_valid.
+      simpl.
+      inversion is_valid_code.
+      - simpl.
+        destruct x0.
+        reflexivity.
+      - simpl.
+        
+      
 
     
-    Set Printing Coercions.
-    Unset Printing Notations.
+    replace (is_state (both_prog (let 'pair _ _ := prod_to_prod_n 1 b in b0)))
+      with
+      ('(_, _) ← (is_state b) ;; is_state b0).
+    2:{
+      clear.
+      destruct b.
+      destruct both_prog.
+      unfold both_prog.
+      unfold ChoiceEquality.is_state.
+      destruct is_state.
+      
+      
+    change (is_state b0) with
+       ('(_, _) ← (is_state b) ;; is_state b0).
     
-    pose (r_bind).
+    unfold prod_to_prod_n at 1 ; fold @prod_to_prod_n.
     
-    apply r_bind.
-    
-    bind_jazz_bind.
-    
-    
-    
-    apply r_assertR.
-    r_assertR.
-    
-    rewrite bind_assoc.
-    rewrite bind_assoc.
+    (* TODO, Sub proofs: *)
+    rewrite random_oracle_query_equation_1.
+    (* TODO, verify proofs: *)
+    rewrite verify_equation_1.
 
-    r_assertR.
+    rewrite prod_both_equation_1.
+    
 
-    ssprove_sync_eq.
+    setoid_rewrite bind_rewrite.
 
     
-Require Import OVN.
+    
 
+
+  
 (* Exec_i_realised *)
 (* {package (Exec_i i j m) ∘ (par ((P_i i b) ∘ (Sigma1.Sigma.Fiat_Shamir ∘ RO1.RO)) *)
 (*                                       (Sigma1.Sigma.Fiat_Shamir ∘ RO1.RO))} *)
-
