ovn/proofs/ssprove/extraction/Hacspec_ovn.v
@@ -26,58 +26,147 @@ Obligation Tactic := (* try timeout 8 *) solve_ssprove_obligations.
 
 (*Not implemented yet? todo(item)*)
 
-Require Import Hacspec_lib.
-Export Hacspec_lib.
+Require Import (* Hacspec_ovn_ *)Hacspec_lib.
+Export (* Hacspec_ovn_ *)Hacspec_lib.
 
-(*Not implemented yet? todo(item)*)
+Class t_Group (Self : choice_type) := {
+  t_group_type : choice_type ;
+  (* t_group_type_t_PartialEq :> t_PartialEq (t_group_type) ; *)
+  (* t_group_type_t_Sized :> t_Sized (t_group_type) ; *)
+  q : forall {L I}, both L I uint_size ;
+  g : t_group_type ;
+  g_pow : forall {L I}, both L I uint_size -> both L I t_group_type ;
+  one : forall {L I}, both L I t_group_type ;
+  prod : forall {L1 L2 I1 I2}, both L1 I1 t_group_type -> both L2 I2 t_group_type -> both (L1 :|: L2) (I1 :|: I2) t_group_type ;
+  div : forall {L1 L2 I1 I2}, both L1 I1 t_group_type -> both L2 I2 t_group_type -> both (L1 :|: L2) (I1 :|: I2) t_group_type ;
+  random_element : t_group_type ;
+}.
 
-Require Import Hacspec_ovn_Schnorr.
-Export Hacspec_ovn_Schnorr.
-
-Notation t_Secret := (t_Q).
-
-Equations sample_uniform : both (fset []) ([interface ]) (t_Q) :=
-  sample_uniform  :=
-    solve_lift (Build_t_Q (ret_both (1 : int32))) : both (fset []) ([interface ]) (t_Q).
+Definition t_eligible_votes : choice_type :=
+  (uint_size).
+Equations Build_t_eligible_votes {L : {fset Location}} {I : Interface} (f_v_id : both L I (uint_size)) : both L I (t_eligible_votes) :=
+  Build_t_eligible_votes f_v_id  :=
+    bind_both f_v_id (fun f_v_id =>
+      solve_lift (ret_both ((f_v_id) : (t_eligible_votes)))) : both L I (t_eligible_votes).
 Fail Next Obligation.
 
-Notation t_public := (t_G).
-
-Notation t_public_key := ((t_G × (t_G × t_G × t_Q × t_Q))).
-
-Equations p_i_init {L1 : {fset Location}} {I1 : Interface} (_ : both L1 I1 ('unit)) : both (L1 :|: fset [commit_loc]) (I1) ((t_G × (t_G × t_G × t_Q × t_Q))) :=
-  p_i_init _  :=
-    letb x := (sample_uniform) : both _ _ (t_Q) in
-    letb y := (Build_t_G (ret_both (1 : int32))) : both _ _ (t_G) in
-    letb zkp := (fiat_shamir_run (prod_b (y,x))) : both _ _ ((t_G × t_G × t_Q × t_Q)) in
-    solve_lift (prod_b (y,zkp)) : both (L1 :|: fset [commit_loc]) (I1) ((t_G × (t_G × t_G × t_Q × t_Q))).
+Equations n : both (fset []) ([interface ]) (uint_size) :=
+  n  :=
+    solve_lift (ret_both (3 : uint_size)) : both (fset []) ([interface ]) (uint_size).
 Fail Next Obligation.
 
-Notation t_N := (nat_mod 0x1a0111ea397fe69a4b1ba7b6434bacd764774b84f38512bf6730d2a0f6b0f6241eabfffeb153ffffb9feffffffffaaab).
-Definition N {L : {fset Location}} {I : Interface} : both L I (t_N) -> both L I (t_N) :=
-  id.
-
-Notation t_pid := (t_N).
-
-Require Import HashMap.
-Export HashMap.
-
-Notation t_public_keys := (t_HashMap (t_N) ((t_G × (t_G × t_G × t_Q × t_Q))) (t_RandomState)).
-
-Equations p_i_construct {L1 : {fset Location}} {I1 : Interface} (m : both L1 I1 (t_HashMap (t_N) ((t_G × (t_G × t_G × t_Q × t_Q))) (t_RandomState))) : both (L1) (I1) ('unit) :=
-  p_i_construct m  :=
-    solve_lift (ret_both (tt : 'unit)) : both (L1) (I1) ('unit).
+Equations v_P : both (fset []) ([interface ]) (nseq t_eligible_votes 3) :=
+  v_P  :=
+    array_from_list [solve_lift (Build_t_eligible_votes (* Build_t_C_eligible_votes *) (ret_both (0 : uint_size)));
+      solve_lift (Build_t_eligible_votes (* Build_t_C_eligible_votes *) (ret_both (1 : uint_size)));
+      solve_lift (Build_t_eligible_votes (* Build_t_C_eligible_votes *) (ret_both (2 : uint_size)))] : both (fset []) ([interface ]) (nseq t_eligible_votes 3).
 Fail Next Obligation.
 
-Equations p_i_vote {L1 : {fset Location}} {I1 : Interface} (v : both L1 I1 ('bool)) : both (L1) (I1) (t_G) :=
-  p_i_vote v  :=
-    solve_lift (Build_t_G (ret_both (1 : int32))) : both (L1) (I1) (t_G).
+Equations select_private_voting_key (G : _) (* `{ t_Sized (G)} *) `{ t_Group (G)} {L1 : {fset Location}} {I1 : Interface} (random : both L1 I1 (uint_size)) : both (L1) (I1) (uint_size) :=
+  select_private_voting_key G random  :=
+    solve_lift (random .% q) : both (L1) (I1) (uint_size).
 Fail Next Obligation.
 
-Equations exec {L1 : {fset Location}} {I1 : Interface} (v : both L1 I1 ('bool)) : both (L1 :|: fset [commit_loc]) (I1) (t_G) :=
-  exec v  :=
-    letb x := (sample_uniform) : both _ _ (t_Q) in
-    letb y := (Build_t_G (ret_both (1 : int32))) : both _ _ (t_G) in
-    letb zkp := (fiat_shamir_run (prod_b (y,x))) : both _ _ ((t_G × t_G × t_Q × t_Q)) in
-    solve_lift (p_i_vote v) : both (L1 :|: fset [commit_loc]) (I1) (t_G).
+Equations v_ZKP (G : _) (* `{ t_Sized (G)} *) `{ t_Group (G)} {L1 : {fset Location}} {I1 : Interface} (xi : both L1 I1 (uint_size)) : both (L1) (I1) (uint_size) :=
+  v_ZKP G xi  :=
+    solve_lift (ret_both (0 : uint_size)) : both (L1) (I1) (uint_size).
+Fail Next Obligation.
+
+Require Import Core.
+
+Equations get_broadcast1 : both (fset []) ([interface ]) ((t_Vec (uint_size) (t_Global) × t_Vec (uint_size) (t_Global))) :=
+  get_broadcast1  :=
+    solve_lift (prod_b (@new _ fset0 fset0,@new _ fset0 fset0)) : both (fset []) ([interface ]) ((t_Vec (uint_size) (t_Global) × t_Vec (uint_size) (t_Global))).
+Fail Next Obligation.
+
+Equations check_valid {L1 : {fset Location}} {I1 : Interface} (zkp : both L1 I1 (uint_size)) : both (L1) (I1) ('bool) :=
+  check_valid zkp  :=
+    solve_lift (ret_both (true : 'bool)) : both (L1) (I1) ('bool).
+Fail Next Obligation.
+
+Equations broadcast1 (G : _) (* `{ t_Sized (G)} *) `{ t_Group (G)} {L1 : {fset Location}} {L2 : {fset Location}} {L3 : {fset Location}} {I1 : Interface} {I2 : Interface} {I3 : Interface} (xi : both L1 I1 (t_group_type)) (zkp : both L2 I2 (uint_size)) (i : both L3 I3 (uint_size)) : both (L1:|:L2:|:L3) (I1:|:I2:|:I3) ('unit) :=
+  broadcast1 G xi zkp i  :=
+    solve_lift (ret_both (tt : 'unit)) : both (L1:|:L2:|:L3) (I1:|:I2:|:I3) ('unit).
+Fail Next Obligation.
+
+Require Import (* Hacspec_ovn_ *)Hacspec_lib.
+Export (* Hacspec_ovn_ *)Hacspec_lib.
+
+Definition prod1_loc {G : _} (* `{ t_Sized (G)} *) `{ t_Group (G)} : Location :=
+  (t_group_type ; 0%nat).
+Equations register_vote (G : _) (* `{ t_Sized (G)} *) `{ t_Group (G)} {L1 : {fset Location}} {L2 : {fset Location}} {I1 : Interface} {I2 : Interface} (i : both L1 I1 (uint_size)) (random : both L2 I2 (uint_size)) : both (L1:|:L2 :|: fset [prod1_loc]) (I1:|:I2) ('unit) :=
+  register_vote G i random  := 
+    letb xi := (select_private_voting_key G random) : both _ _ (uint_size) in
+    letb _ := (broadcast1 G (g_pow xi) (v_ZKP G xi) i) : both _ _ ('unit) in
+    letb _ := (ret_both (tt : 'unit)) : both _ _ ('unit) in
+    letb '(gs,zkps) := (get_broadcast1) : both _ _ ((t_Vec (uint_size) (t_Global) × t_Vec (uint_size) (t_Global))) in
+    (* letb _ := (other loop todo(term)) : both _ _ ('unit) in *) (* TODO LOOP *)
+    letbm prod1 loc(prod1_loc) := (one) : both _ _ (t_group_type) in
+    letb prod1 := (foldi_both (into_iter (Build_t_Range (ret_both (1 : uint_size)) (i .- (ret_both (1 : uint_size))))) (fun {L I _ _} =>fun j =>
+        (ssp (fun prod1 =>
+                solve_lift (prod prod1 (g_pow (gs.a[j])))) )) prod1) : both _ _ (t_group_type) in
+    letb prod2 := (one) : both _ _ (t_group_type) in
+    letb prod1 := (foldi_both (into_iter (Build_t_Range (i .+ (ret_both (1 : uint_size)))n)) (fun {L I _ _} =>fun j =>
+        (ssp (fun prod1 =>
+          solve_lift (prod prod1 (g_pow (gs.a[j])))) )) prod1) : both _ _ (t_group_type) in
+    letb Yi := (div prod1 prod2) : both _ _ (t_group_type) in
+      solve_lift (ret_both (tt : 'unit)) : both (L1:|:L2 :|: fset [prod1_loc]) (I1:|:I2) ('unit).
+Next Obligation.
+  admit.
+Admitted.
+Next Obligation.
+  admit.
+Admitted.
+Fail Next Obligation.
+
+Equations v_ZKP_one_out_of_two {L1 : {fset Location}} {I1 : Interface} (vi : both L1 I1 ('bool)) : both (L1) (I1) (uint_size) :=
+  v_ZKP_one_out_of_two vi  :=
+    solve_lift (ret_both (32 : uint_size)) : both (L1) (I1) (uint_size).
+Fail Next Obligation.
+
+Equations broadcast2 (G : _) (* `{ t_Sized (G)} *) `{ t_Group (G)} {L1 : {fset Location}} {L2 : {fset Location}} {L3 : {fset Location}} {I1 : Interface} {I2 : Interface} {I3 : Interface} (g_pow_xiyi : both L1 I1 (t_group_type)) (g_pow_vi : both L2 I2 (t_group_type)) (g_pow_vi_zkp : both L3 I3 (uint_size)) : both (L1:|:L2:|:L3) (I1:|:I2:|:I3) ('unit) :=
+  broadcast2 G g_pow_xiyi g_pow_vi g_pow_vi_zkp  :=
+    solve_lift (ret_both (tt : 'unit)) : both (L1:|:L2:|:L3) (I1:|:I2:|:I3) ('unit).
+Fail Next Obligation.
+
+Equations get_broadcast2 (G : _) (* `{ t_Sized (G)} *) `{ t_Group (G)} : both (fset []) ([interface ]) ((t_Vec (t_group_type) (t_Global) × t_Vec (t_group_type) (t_Global) × t_Vec (uint_size) (t_Global))) :=
+  get_broadcast2 G  :=
+    solve_lift (prod_b (@new _ fset0 fset0,@new _ fset0 fset0,@new _ fset0 fset0)) : both (fset []) ([interface ]) ((t_Vec (t_group_type) (t_Global) × t_Vec (t_group_type) (t_Global) × t_Vec (uint_size) (t_Global))).
+Fail Next Obligation.
+
+Equations cast_vote (G : _) (* `{ t_Sized (G)} *) `{ t_Group (G)} {L1 : {fset Location}} {L2 : {fset Location}} {L3 : {fset Location}} {I1 : Interface} {I2 : Interface} {I3 : Interface} (xi : both L1 I1 (uint_size)) (yi : both L2 I2 (uint_size)) (vi : both L3 I3 ('bool)) : both (L1:|:L2:|:L3) (I1:|:I2:|:I3) ('unit) :=
+  cast_vote G xi yi vi  :=
+    letb _ := (broadcast2 G (g_pow (xi .* yi)) (g_pow (ifb vi
+      then ret_both (1 : uint_size)
+      else ret_both (0 : uint_size))) (v_ZKP_one_out_of_two vi)) : both _ _ ('unit) in
+    letb _ := (ret_both (tt : 'unit)) : both _ _ ('unit) in
+    solve_lift (ret_both (tt : 'unit)) : both (L1:|:L2:|:L3) (I1:|:I2:|:I3) ('unit).
+Fail Next Obligation.
+
+Definition vote_result_loc {G : _} (* `{ t_Sized (G)} *) `{ t_Group (G)} : Location :=
+  (t_group_type ; 2%nat).
+Definition tally_loc {G : _} (* `{ t_Sized (G)} *) `{ t_Group (G)} : Location :=
+  (uint_size ; 1%nat).
+Definition into_iter_zip {L I A B} (x : both L I (chList (A × B))) : both L I (chList A) * both L I (chList B). Admitted.
+Equations tally_votes (G : _) (* `{ t_Sized (G)} *) `{ t_Group (G)} : both (fset [tally_loc; vote_result_loc]) ([interface ]) (uint_size) :=
+  tally_votes G  :=
+    letb '(g_pow_xi_yi,g_pow_vi,zkps) := (get_broadcast2 G) : both _ _ ((t_Vec (t_group_type) (t_Global) × t_Vec (t_group_type) (t_Global) × t_Vec (uint_size) (t_Global))) in
+    (* letb _ := (other loop todo(term)) : both _ _ ('unit) in *) (* TODO Loop *)
+    letbm vote_result loc(vote_result_loc) := (one) : both _ _ (t_group_type) in
+    (* letb vote_result := (foldi_both (into_iter_zip ((lift2_both (fun (x : chList _) (y : chList _) => seq.zip x y : chList (chProd _ _))) (into_iter g_pow_xi_yi) g_pow_vi)) (fun {L I _ _} =>fun '(gxiyi,gvi) => *)
+    (*     (ssp (fun vote_result => *)
+      (*       solve_lift (prod vote_result (prod gxiyi gvi))) )) vote_result) : both _ _ (t_group_type) in *)
+      (* TODO for_loop *)
+    letbm tally loc(tally_loc) := (ret_both (0 : uint_size)) : both _ _ (uint_size) in
+    (* letb tally := (foldi_both (into_iter (Build_t_Range (ret_both (1 : uint_size))n)) (fun {L I _ _} =>fun i => *)
+    (*     (ssp (fun tally => *)
+    (*       ifb solve_lift ((g_pow tally) <> vote_result) *)
+    (*       then ControlFlow_Continue (letb _ := (tally .+ (ret_both (1 : uint_size))) : both _ _ ('unit) in *)
+    (*         solve_lift (ret_both (tt : 'unit))) *)
+    (*       else letb hoist1 := (v_Break tally) : both _ _ (t_Never) in *)
+    (*         ControlFlow_Continue (letb _ := (never_to_any hoist1) : both _ _ ('unit) in *)
+      (*         tally)) )) tally) : both _ _ ('unit) in *)
+      (* TODO for_loop *)
+      solve_lift tally : both (fset [tally_loc; vote_result_loc]) ([interface ]) (uint_size).
+Admit Obligations.
 Fail Next Obligation.
