ovn/proofs/ssprove/extraction/HashMap.v
@@ -48,8 +48,20 @@ Inductive random_state :=
   t_RandomState.
 Definition t_HashMap A B (_ : random_state) := chMap A B.
 
-Axiom insert : forall {L1 L2 L3 I1 I2 I3 A B}, both L1 I1 (t_HashMap A B t_RandomState) -> both L2 I2 A -> both L3 I3 B -> both (L1 :|: L2 :|: L3) (I1 :|: I2 :|: I3) (t_Option B × t_HashMap A B t_RandomState).
-Axiom get :  forall {L1 L2 I1 I2 A B}, both L1 I1 (t_HashMap A B t_RandomState) -> both L2 I2 A -> both (L1 :|: L2) (I1 :|: I2) (t_Option B).
+Equations insert : forall {L1 L2 L3 I1 I2 I3} {A B : choice_type}, both L1 I1 (t_HashMap A B t_RandomState) -> both L2 I2 A -> both L3 I3 B -> both (L1 :|: L2 :|: L3) (I1 :|: I2 :|: I3) (t_Option B × t_HashMap A B t_RandomState) :=
+  insert m i v :=
+    bind_both m (fun m' =>
+    bind_both i (fun i' =>
+    bind_both v (fun v' =>
+    solve_lift ret_both (
+      (Some v', setm m' (chElement_ordType_ce_to_ce A i') v')
+                 : chOption B × t_HashMap A B _)))).
 
-Axiom new :  forall {L I A B}, both L I (t_HashMap A B t_RandomState).
+Equations get {L1 L2 I1 I2} {A B} (m : both L1 I1 (t_HashMap A B t_RandomState)) (i : both L2 I2 A) : both (L1 :|: L2) (I1 :|: I2) (t_Option B) :=
+  get m i :=
+    bind_both m (fun m' =>
+    bind_both i (fun i' =>
+    solve_lift ret_both (getm m' (chElement_ordType_ce_to_ce A i') : chOption B))).
 
+Equations new {L I A B} : both L I (t_HashMap A B t_RandomState) :=
+  new := (solve_lift ret_both emptym). (* (fmap (s:=[]) _ : chMap _ _) *)
